

CHAPTER – 12

Discrete MathematicsExercise 12.1

1. Determine whether $*$ is a binary operation on the sets given below.

(i) $a * b = a \cdot |b|$ on \mathbb{R}

Solution:

Let $a, b \in \mathbb{R}$

$$|b| \in \mathbb{R}$$

$$a \cdot |b| \in \mathbb{R}$$

$$a * b \in \mathbb{R}$$

Hence $*$ is binary on \mathbb{R} .

(ii) $a * b = \min(a, b)$ on $A = \{1, 2, 3, 4, 5\}$

Solution:

Let $a, b \in A$

$\min(a, b)$ is either a or b , which belongs to A .

$$a * b \in A$$

Hence $*$ is binary on A .

(iii) $(a * b) = a\sqrt{b}$ is binary on \mathbb{R} .

Solution:

Let $a, b \in \mathbb{R}$

$$\sqrt{b} \notin \mathbb{R} \quad (\because b = -1 \text{ then } \sqrt{-1} \notin \mathbb{R})$$

$$a\sqrt{b} \notin \mathbb{R}$$

$$a * b \notin \mathbb{R}$$

Hence $*$ not binary on \mathbb{R} .

2. On \mathbb{Z} , define $*$ by $(m * n) = m^n + n^m: \forall m, n \in \mathbb{Z}$. Is $*$ binary on \mathbb{Z} ?

Solution:

Let $m, n \in \mathbb{Z}$

$$m^n \notin \mathbb{Z} \text{ (if } n < 0) \quad \left(m^{-1} = \frac{1}{m} \notin \mathbb{Z}\right)$$

$$m^n + n^m \notin \mathbb{Z}$$

$$m * n \notin \mathbb{Z}$$

Hence $*$ is not binary on \mathbb{Z} .

3. Let $*$ be defined on \mathbb{R} by $(a * b) = a + b + ab - 7$. Is $*$ binary on \mathbb{R} ? If so, find $3 * \left(\frac{-7}{15}\right)$.

Solution:

Given $a * b = a + b + ab - 7$

Let $a, b \in \mathbb{R}$

$$a + b \in \mathbb{R}$$

$$ab \in \mathbb{R}$$

$$-7 \in \mathbb{R}$$

$$a + b + ab - 7 \in \mathbb{R}$$

$$a * b \in \mathbb{R}$$

Hence $*$ is binary on \mathbb{R} .

$$\begin{aligned} 3 * \left(-\frac{7}{15}\right) &= 3 - \frac{7}{15} - \frac{21}{15} - 7 \\ &= -4 - \frac{28}{15} \\ &= \frac{-60-28}{15} \end{aligned}$$

$$3 * \left(-\frac{7}{15}\right) = -\frac{88}{15}$$

4. Let $A = \{a + \sqrt{5}b : a, b \in \mathbb{Z}\}$. Check whether the usual multiplication is a binary operation on A .

Solution:

Let $a + \sqrt{5}b, c + \sqrt{5}d \in A$, where $a, b, c, d \in \mathbb{Z}$

$$(a + \sqrt{5}b)(c + \sqrt{5}d) = ac + \sqrt{5}ad + \sqrt{5}bc + 5bd$$

$$= (ac + 5bd) + \sqrt{5}(ad + bc) \in A$$

Hence usual multiplication is binary on A .

5. (i) Define an operation $*$ on \mathbb{Q} as follows:

$a * b = \left(\frac{a+b}{2}\right); a, b \in \mathbb{Q}$. Examine the closure, commutative, and associative properties satisfied by $*$ on \mathbb{Q} .

Solution:

Given $a * b = \frac{a+b}{2}$

Closure Property:

Let $a, b \in \mathbb{Q}$

$$a + b \in \mathbb{Q}$$

$$\frac{a+b}{2} \in \mathbb{Q}$$

$$a * b \in \mathbb{Q}$$

Hence closure property is true.

Commutative Property:

Let $a, b \in \mathbb{Q}$

$$a * b = \frac{a+b}{2}$$

$$= \frac{b+a}{2}$$

$$a * b = b * a$$

Hence commutative property is true.

Associative Property:

Let $a, b, c \in \mathbb{Q}$

$$a * (b * c) = a * \left(\frac{b+c}{2}\right)$$

$$= \frac{a + \left(\frac{b+c}{2}\right)}{2}$$

$$a * (b * c) = \frac{2a+b+c}{4} \text{-----(1)}$$

$$(a * b) * c = \left(\frac{a+b}{2}\right) * c$$

$$= \frac{\left(\frac{a+b}{2}\right) + c}{2}$$

$$(a * b) * c = \frac{a+b+2c}{4} \text{-----(2)}$$

From (1) and (2) we have

$$a * (b * c) \neq (a * b) * c$$

Hence associative property is not true.

(ii) Define an operation $*$ on \mathbb{Q} as follows: $a * b = \left(\frac{a+b}{2}\right); a, b \in \mathbb{Q}$. Examine the existence of identity and the existence of inverse for the operation $*$ on \mathbb{Q} .

Solution:

$$\text{Given } a * b = \frac{a+b}{2}$$

Existence of Identity Property:

Let $a \in \mathbb{Q}$

By definition, $a * e = a$

$$\frac{a+e}{2} = a$$

$$a + e = 2a$$

$$e = a, \text{ which is not unique}$$

Hence identity property fails.

Existence of Inverse Property:

$*$ has no identity element.

Hence $*$ has no inverse.

6. Fill in the following table so that the binary operation $*$ on $A = \{a, b, c\}$ is commutative.

$*$	a	b	c
a	b		
b	c	b	a
c	a		c

Solution:

Given $*$ is commutative.

$*$	a	b	c
a	b	c	a
b	c	b	a
c	a	a	c

From table:

$$b * a = c = a * b$$

$$b * c = a = c * b$$

$$c * a = a = a * c$$

7. Consider the binary operation $*$ defined on the set $A = \{a, b, c, d\}$ by the following table:

$*$	a	b	c	d
a	a	c	b	d
b	d	a	b	c
c	c	d	a	a
d	d	b	a	c

Is it commutative and associative?

Solution:

Commutative:

From table, $a * b = c$

$$b * a = d$$

$$a * b \neq b * a$$

Hence $*$ is not commutative on A .

Associative:

$$(a * b) * c = c * c = a \text{-----(1)}$$

$$a * (b * c) = a * b = c \text{ } (\because b * c = b) \text{-----(2)}$$

From (1) and (2) we have

$$(a * b) * c \neq a * (b * c)$$

Hence $*$ is not associative on A .

Hint: $a \vee b = \max\{a, b\}; a \wedge b = \min\{a, b\}$

8. Let $A = \begin{bmatrix} 1 & 0 & 1 & 0 \\ 0 & 1 & 0 & 1 \\ 1 & 0 & 0 & 1 \end{bmatrix}, B = \begin{bmatrix} 0 & 1 & 0 & 1 \\ 1 & 0 & 1 & 0 \\ 1 & 0 & 0 & 1 \end{bmatrix}$ and

$C = \begin{bmatrix} 1 & 1 & 0 & 1 \\ 0 & 1 & 1 & 0 \\ 1 & 1 & 1 & 1 \end{bmatrix}$ be any three Boolean matrices of the same type. Find (i) $A \vee B$ (ii) $A \wedge B$ (iii) $(A \vee B) \wedge C$ (iv) $(A \wedge B) \vee C$.

Solution:

$$(i) \quad A \vee B = \begin{bmatrix} 1 & 0 & 1 & 0 \\ 0 & 1 & 0 & 1 \\ 1 & 0 & 0 & 1 \end{bmatrix} \vee \begin{bmatrix} 0 & 1 & 0 & 1 \\ 1 & 0 & 1 & 0 \\ 1 & 0 & 0 & 1 \end{bmatrix}$$

$$A \vee B = \begin{bmatrix} 1 \vee 0 & 0 \vee 1 & 1 \vee 0 & 0 \vee 1 \\ 0 \vee 1 & 1 \vee 0 & 0 \vee 1 & 1 \vee 0 \\ 1 \vee 1 & 0 \vee 0 & 0 \vee 0 & 1 \vee 1 \end{bmatrix}$$

$$\begin{aligned}
 A \vee B &= \begin{bmatrix} 1 & 1 & 1 & 1 \\ 1 & 1 & 1 & 1 \\ 1 & 0 & 0 & 1 \end{bmatrix} \\
 \text{(ii)} \quad A \wedge B &= \begin{bmatrix} 1 \wedge 0 & 0 \wedge 1 & 1 \wedge 0 & 0 \wedge 1 \\ 0 \wedge 1 & 1 \wedge 0 & 0 \wedge 1 & 1 \wedge 0 \\ 1 \wedge 1 & 0 \wedge 0 & 0 \wedge 0 & 1 \wedge 1 \end{bmatrix} \\
 A \wedge B &= \begin{bmatrix} 0 & 0 & 0 & 0 \\ 0 & 0 & 0 & 0 \\ 1 & 0 & 0 & 1 \end{bmatrix} \\
 \text{(iii)} \quad (A \vee B) \wedge C &= \begin{bmatrix} 1 \wedge 1 & 1 \wedge 1 & 1 \wedge 0 & 1 \wedge 1 \\ 1 \wedge 0 & 1 \wedge 1 & 1 \wedge 1 & 1 \wedge 0 \\ 1 \wedge 1 & 0 \wedge 1 & 0 \wedge 1 & 1 \wedge 1 \end{bmatrix} \\
 (A \vee B) \wedge C &= \begin{bmatrix} 1 & 1 & 0 & 1 \\ 0 & 1 & 1 & 0 \\ 1 & 0 & 0 & 1 \end{bmatrix} \\
 \text{(iv)} \quad (A \wedge B) \vee C &= \begin{bmatrix} 0 \vee 1 & 0 \vee 1 & 0 \vee 0 & 0 \vee 1 \\ 0 \vee 0 & 0 \vee 1 & 0 \vee 1 & 0 \vee 0 \\ 1 \vee 1 & 0 \vee 1 & 0 \vee 1 & 1 \vee 1 \end{bmatrix} \\
 (A \wedge B) \vee C &= \begin{bmatrix} 1 & 1 & 0 & 1 \\ 0 & 1 & 1 & 0 \\ 1 & 1 & 1 & 1 \end{bmatrix}
 \end{aligned}$$

9. (i) Let $M = \left\{ \begin{pmatrix} x & x \\ x & x \end{pmatrix} : x \in \mathbb{R} - \{0\} \right\}$ and let $*$ be the matrix multiplication. Determine whether M is closed under $*$. If so, examine the commutative and associative properties satisfied by $*$ on M .

Solution:

$$\text{Given } M = \left\{ \begin{pmatrix} x & x \\ x & x \end{pmatrix} : x \in \mathbb{R} - \{0\} \right\}$$

Closure:

$$\text{Let } A = \begin{bmatrix} x & x \\ x & x \end{bmatrix}, B = \begin{bmatrix} y & y \\ y & y \end{bmatrix} \in M \text{ where } x, y \in \mathbb{R} - \{0\}$$

$$\begin{aligned}
 A * B &= \begin{bmatrix} x & x \\ x & x \end{bmatrix} * \begin{bmatrix} y & y \\ y & y \end{bmatrix} \\
 &= \begin{bmatrix} xy + xy & xy + xy \\ xy + xy & xy + xy \end{bmatrix}
 \end{aligned}$$

$$A * B = \begin{bmatrix} 2xy & 2xy \\ 2xy & 2xy \end{bmatrix} \in M \text{ where } 2xy \in \mathbb{R} - \{0\}$$

Hence $*$ is binary on M .

Commutative property:

$$\begin{aligned}
 B * A &= \begin{bmatrix} y & y \\ y & y \end{bmatrix} * \begin{bmatrix} x & x \\ x & x \end{bmatrix} \\
 &= \begin{bmatrix} 2yx & 2yx \\ 2yx & 2yx \end{bmatrix} \\
 &= \begin{bmatrix} 2xy & 2xy \\ 2xy & 2xy \end{bmatrix}
 \end{aligned}$$

$$B * A = A * B$$

Hence commutative property is true.

Associative property:

$$\text{Let } A = \begin{bmatrix} x & x \\ x & x \end{bmatrix}, B = \begin{bmatrix} y & y \\ y & y \end{bmatrix}, C = \begin{bmatrix} z & z \\ z & z \end{bmatrix} \in M$$

$$\begin{aligned}
 A * (B * C) &= \begin{bmatrix} x & x \\ x & x \end{bmatrix} * \left(\begin{bmatrix} y & y \\ y & y \end{bmatrix} * \begin{bmatrix} z & z \\ z & z \end{bmatrix} \right) \\
 &= \begin{bmatrix} x & x \\ x & x \end{bmatrix} * \begin{bmatrix} 2yz & 2yz \\ 2yz & 2yz \end{bmatrix} \\
 &= \begin{bmatrix} 2xyz + 2xyz & 2xyz + 2xyz \\ 2xyz + 2xyz & 2xyz + 2xyz \end{bmatrix} \\
 &= \begin{bmatrix} 4xyz & 4xyz \\ 4xyz & 4xyz \end{bmatrix} \quad \text{-----(1)}
 \end{aligned}$$

$$\begin{aligned}
 (A * B) * C &= \left(\begin{bmatrix} x & x \\ x & x \end{bmatrix} * \begin{bmatrix} y & y \\ y & y \end{bmatrix} \right) * \begin{bmatrix} z & z \\ z & z \end{bmatrix} \\
 &= \begin{bmatrix} 2xy & 2xy \\ 2xy & 2xy \end{bmatrix} * \begin{bmatrix} z & z \\ z & z \end{bmatrix} \\
 &= \begin{bmatrix} 4xyz & 4xyz \\ 4xyz & 4xyz \end{bmatrix} \quad \text{-----(2)}
 \end{aligned}$$

From (1) and (2) we have

$$A * (B * C) = (A * B) * C$$

Hence Associative property is true.

(ii) Let $M = \left\{ \begin{pmatrix} x & x \\ x & x \end{pmatrix} : x \in \mathbb{R} - \{0\} \right\}$ and let $*$ be the matrix multiplication. Determine whether M is closed under $*$. If so, examine the existence of identity, existence of inverse properties for the operation $*$ on M .

Solution:

$$\text{Given } M = \left\{ \begin{pmatrix} x & x \\ x & x \end{pmatrix} : x \in \mathbb{R} - \{0\} \right\}$$

Existence of Identity property:

$$\text{Let } A = \begin{bmatrix} x & x \\ x & x \end{bmatrix} \in M \text{ where } x \in \mathbb{R} - \{0\}$$

$$\text{Let } E = \begin{bmatrix} e & e \\ e & e \end{bmatrix} \text{ be the identity element.}$$

By definition, $A * E = A$

$$\begin{bmatrix} x & x \\ x & x \end{bmatrix} * \begin{bmatrix} e & e \\ e & e \end{bmatrix} = \begin{bmatrix} x & x \\ x & x \end{bmatrix}$$

$$\begin{bmatrix} 2xe & 2xe \\ 2xe & 2xe \end{bmatrix} = \begin{bmatrix} x & x \\ x & x \end{bmatrix}$$

$$2xe = x$$

$$2e = 1$$

$$e = \frac{1}{2} \in \mathbb{R} - \{0\}$$

$$E = \begin{bmatrix} \frac{1}{2} & \frac{1}{2} \\ \frac{1}{2} & \frac{1}{2} \end{bmatrix} \in M$$

Similarly, $E * A = A$

Hence $E = \begin{bmatrix} \frac{1}{2} & \frac{1}{2} \\ \frac{1}{2} & \frac{1}{2} \end{bmatrix}$ is the identity element.

Existence of Inverse property:

Let $A = \begin{bmatrix} x & x \\ x & x \end{bmatrix} \in M$ where $x \in \mathbb{R} - \{0\}$

Let $B = \begin{bmatrix} y & y \\ y & y \end{bmatrix}$ be the inverse of A .

By definition, $A * B = E$

$$\begin{bmatrix} x & x \\ x & x \end{bmatrix} * \begin{bmatrix} y & y \\ y & y \end{bmatrix} = \begin{bmatrix} e & e \\ e & e \end{bmatrix}$$

$$\begin{bmatrix} 2xy & 2xy \\ 2xy & 2xy \end{bmatrix} = \begin{bmatrix} \frac{1}{2} & \frac{1}{2} \\ \frac{1}{2} & \frac{1}{2} \end{bmatrix}$$

$$2xy = \frac{1}{2}$$

$$y = \frac{1}{4x} \in \mathbb{R} - \{0\}$$

Hence the inverse of A is $\begin{bmatrix} \frac{1}{4x} & \frac{1}{4x} \\ \frac{1}{4x} & \frac{1}{4x} \end{bmatrix}$.

10. (i) Let A be $\mathbb{Q} \setminus \{1\}$. Define $*$ on A by $x * y = x + y - xy$. Is $*$ binary on A ? If so, examine the commutative and associative properties satisfied by $*$ on A .

Solution:

Given $A = \mathbb{Q} \setminus \{1\}$

$$x * y = x + y - xy$$

Closure property:

Let $x, y \in \mathbb{Q} \setminus \{1\}$.

$$x \neq 1 ; \quad y \neq 1$$

$$x - 1 \neq 0 ; \quad y - 1 \neq 0$$

$$(x - 1)(y - 1) \neq 0$$

$$xy - x - y + 1 \neq 0$$

$$x + y - xy \neq 1$$

$$x * y \neq 1$$

$$x * y \in A \quad (\because x, y \in \mathbb{Q})$$

Hence $*$ is binary on A .

Commutative property:

Let $x, y \in A$

$$x * y = x + y - xy$$

$$= y + x - yx$$

$$x * y = y * x$$

Hence commutative property is true.

Associative property:

Let $x, y, z \in A$

$$\begin{aligned} x * (y * z) &= x * (y + z - yz) \\ &= x + y + z - yz - x(y + z - yz) \\ &= x + y + z - yz - xy - xz + xyz \quad \text{-----(1)} \end{aligned}$$

$$\begin{aligned} (x * y) * z &= (x + y - xy) * z \\ &= x + y - xy + z - (x + y - xy)z \\ &= x + y + z - xy - xz - yz + xyz \quad \text{-----(2)} \end{aligned}$$

From (1) and (2) we have

$$x * (y * z) = (x * y) * z$$

Hence associative property is true.

(ii) Let A be $\mathbb{Q} \setminus \{1\}$. Define $*$ on A by $x * y = x + y - xy$. Is $*$ binary on A ? If so, examine the existence of identity, existence of inverse properties for the operation $*$ on A .

Solution:

Given $A = \mathbb{Q} \setminus \{1\}$

$$x * y = x + y - xy$$

Existence of Identity property:

Let $x \in A$

By definition, $x * e = x$

$$x + e - xe = x$$

$$e - xe = 0$$

$$e(1 - x) = 0$$

$$e = 0 \quad (\because x \neq 1)$$

\therefore The Identity element is $e = 0 \in A$.

Thus identity property is satisfied.

Existence of Inverse property:

Let $x \in A$

By definition, $x * x^{-1} = e$

$$x + x^{-1} - xx^{-1} = 0$$

$$x + x^{-1}(1 - x) = 0$$

$$x^{-1}(1 - x) = -x$$

$$x^{-1} = \frac{-x}{1-x} \in \mathbb{Q} \setminus \{1\} \quad (\because x \neq 1)$$

\therefore The Inverse element is $x^{-1} = \frac{-x}{1-x} \in A$

Hence inverse property is satisfied.

Exercise 12.2

1. Let P : Jupiter is a planet and q : India is an island be any two simple statements. Give verbal sentence describing each of the following statements.

(i) $\neg p$ (ii) $p \wedge \neg q$ (iii) $\neg p \vee q$ (iv) $p \rightarrow \neg q$ (v) $p \leftrightarrow q$

Solutions:

(i) $\neg p$: Jupiter is not a planet

(ii) $p \wedge \neg q$: Jupiter is a planet and India is not an island

(iii) $\neg p \vee q$: Jupiter is not a planet or India is an island

(iv) $p \rightarrow \neg q$: If Jupiter is a planet then India is not an island

(v) $p \leftrightarrow q$: Jupiter is a planet if and only if India is an island

2. Write each of the following sentences in symbolic form using statement variables p and q .

(i) 19 is not a prime number and all the angles of a triangle are equal.

(ii) 19 is a prime number or all the angles of a triangle are not equal.

(iii) 19 is a prime number and all the angles of a triangle are equal.

(iv) 19 is not a prime number.

Solutions:

p : 19 is a prime number

q : All the angles of a triangle are equal

(i) $\neg p \wedge q$

(ii) $p \vee \neg q$

(iii) $p \wedge q$

(iv) $\neg p$

Hint: Symbolic form

“then” (\rightarrow) “or” (\vee) “and” (\wedge)

3. Determine the truth value of each of the following statements

(i) If $6 + 2 = 5$, then the milk is white.

(ii) China is in Europe or $\sqrt{3}$ is an integer.

(iii) It is not true that $5 + 5 = 9$ or Earth is a planet.

(iv) 11 is a prime number and all the sides of a rectangle are equal.

Solutions:

S. No	Statement	Symbolic form	Conclusion
(i)	If $6 + 2 = 5$, then the milk is white	$F \rightarrow T$	T
(ii)	China is in Europe or $\sqrt{3}$ is an integer	$F \vee F$	F
(iii)	It is not true that $5 + 5 = 9$ or Earth is a planet	$T \vee T$	T
(iv)	11 is a prime number and all the sides of a rectangle are equal	$T \wedge F$	F

Hint: Any declarative sentence is called statement or a ‘Proposition’ which is either true or false but not both.

4. Which one of the following sentences is a proposition?

(i) $4 + 7 = 12$ (ii) What are you doing? (iii) $3^n \leq 81, n \in \mathbb{N}$ (iv) Peacock is our national bird (v) How tall this mountain is!

Solutions:

(i) Proposition

(ii) Not a proposition (It is interrogative)

(iii) Proposition

(iv) Proposition

(v) Not a proposition (It is Exclamatory)

Hint: (i) Converse statement $q \rightarrow p$

(ii) Inverse statement $\neg p \rightarrow \neg q$

(iii) Contrapositive statement $\neg q \rightarrow \neg p$

5. Write the converse, inverse, and contrapositive of each of the following implication.

(i) If x and y are numbers such that $x = y$, then $x^2 = y^2$

Solution:

p : x and y are numbers such that $x = y$

q : $x^2 = y^2$

Converse: $q \rightarrow p$

\Rightarrow If $x^2 = y^2$ then $x = y$

Inverse: $\neg p \rightarrow \neg q$

\Rightarrow If $x \neq y$ then $x^2 \neq y^2$

Contrapositive: $\neg q \rightarrow \neg p$

\Rightarrow If $x^2 \neq y^2$ then $x \neq y$

(ii) If a quadrilateral is a square then it is rectangle

Solution:

p : A quadrilateral is a square

q : A quadrilateral is rectangle

Converse: $q \rightarrow p$

If a quadrilateral is a rectangle then it is a square.

Inverse: $\neg p \rightarrow \neg q$

If a quadrilateral is not a square then it is not a rectangle.

Contrapositive: $\neg q \rightarrow \neg p$

If a quadrilateral is not an rectangle then it is not a square.

6. Construct the truth table for the following statements.

(i) $\neg p \wedge \neg q$

Solution:

p	q	$\neg p$	$\neg q$	$\neg p \wedge \neg q$
T	T	F	F	F
T	F	F	T	F
F	T	T	F	F
F	F	T	T	T

(ii) $\neg(p \wedge \neg q)$

Solution:

p	q	$\neg q$	$p \wedge \neg q$	$\neg(p \wedge \neg q)$
T	T	F	F	T
T	F	T	T	F
F	T	F	F	T
F	F	T	F	T

(iii) $(p \vee q) \vee \neg q$

Solution:

p	q	$\neg q$	$p \vee q$	$(p \vee q) \vee \neg q$
T	T	F	T	T
T	F	T	T	T
F	T	F	T	T
F	F	T	F	T

(iv) $(\neg p \rightarrow r) \wedge (p \leftrightarrow q)$

Solution:

p	q	r	$\neg p$	$s: \neg p \rightarrow r$	$t: p \leftrightarrow q$	$s \wedge t$
T	T	T	F	T	T	T
T	T	F	F	T	T	T
T	F	T	F	T	F	F
T	F	F	F	T	F	F
F	T	T	T	T	F	F
F	T	F	T	F	F	F
F	F	T	T	T	T	T
F	F	F	T	F	T	F

7. Verify whether the following compound propositions are tautologies or contradictions or contingency

(i) $(p \wedge q) \wedge \neg(p \vee q)$

Solution:

p	q	$s: p \wedge q$	$t: p \vee q$	$\neg t$	$s \wedge \neg t$
T	T	T	T	F	F
T	F	F	T	F	F
F	T	F	T	F	F
F	F	F	F	T	F

This is a contradiction.

(ii) $((p \vee q) \wedge \neg p) \rightarrow q$

Solution:

p	q	$s: p \vee q$	$t: \neg p$	$r: s \wedge t$	$r \rightarrow q$
T	T	T	F	F	T
T	F	T	F	F	T
F	T	T	T	T	T
F	F	F	T	F	T

It is a tautology.

(iii) $(p \rightarrow q) \leftrightarrow (\neg p \rightarrow q)$

Solution:

p	q	$s: p \rightarrow q$	$t: \neg p$	$r: \neg p \rightarrow q$	$s \leftrightarrow r$
T	T	T	F	T	T
T	F	F	F	T	F
F	T	T	T	T	T
F	F	T	T	F	F

Hence It is contingency.

(iv) $((p \rightarrow q) \wedge (q \rightarrow r)) \rightarrow (p \rightarrow r)$

Solution:

p	q	r	$s: p \rightarrow q$	$t: q \rightarrow r$	$u: p \rightarrow r$	$w: s \wedge t$	$w \rightarrow u$
T	T	T	T	T	T	T	T
T	T	F	T	F	F	F	T
T	F	T	F	T	T	F	T
T	F	F	F	T	F	F	T
F	T	T	T	T	T	T	T
F	T	F	T	F	T	F	T
F	F	T	T	T	T	T	T
F	F	F	T	T	T	T	T

It is a tautology.

8. Show that (i) $\neg(p \wedge q) \equiv \neg p \vee \neg q$

Solution:

p	q	$s: p \wedge q$	$\neg s$	$\neg p$	$\neg q$	$\neg p \vee \neg q$
T	T	T	F	F	F	F
T	F	F	T	F	T	T
F	T	F	T	T	F	T
F	F	F	T	T	T	T

From the table, $\neg(p \wedge q) \equiv \neg p \vee \neg q$

(ii) $\neg(p \rightarrow q) \equiv p \wedge \neg q$

Solution:

p	q	$s: p \rightarrow q$	$\neg s$	$\neg q$	$p \wedge \neg q$
T	T	T	F	F	F
T	F	F	T	T	T
F	T	T	F	F	F
F	F	T	F	T	F

From the table, $\neg(p \rightarrow q) \equiv p \wedge \neg q$

9. Prove that $q \rightarrow p \equiv \neg p \vee \neg q$

Solution:

p	q	$q \rightarrow p$	$\neg p$	$\neg q$	$\neg p \vee \neg q$
T	T	T	F	F	T
T	F	T	F	T	T
F	T	F	T	F	F
F	F	T	T	T	T

From the table, $q \rightarrow p \equiv \neg p \vee \neg q$

10. Show that $p \rightarrow q$ and $q \rightarrow p$ are not equivalent.

Solution:

p	q	$p \rightarrow q$	$q \rightarrow p$
T	T	T	T
T	F	F	T
F	T	T	F
F	F	T	T

From the table, $p \rightarrow q \neq q \rightarrow p$.

11. Show that $\neg(p \leftrightarrow q) \equiv p \leftrightarrow \neg q$

Solution:

p	q	$s: p \leftrightarrow q$	$\neg s$	$\neg q$	$p \leftrightarrow \neg q$
T	T	T	F	F	F
T	F	F	T	T	T
F	T	F	T	F	T
F	F	T	F	T	F

From the table, $\neg(p \leftrightarrow q) \equiv p \leftrightarrow \neg q$

Hint: $p \rightarrow q \equiv \neg p \vee q$

12. Check whether the statement $p \rightarrow (q \rightarrow p)$ is a tautology or a contradiction without using the truth table.

Solution:

$$\begin{aligned}
 p \rightarrow (q \rightarrow p) &\equiv p \rightarrow (\neg q \vee p) \\
 &\equiv \neg p \vee (\neg q \vee p) \\
 &\equiv \neg p \vee (p \vee \neg q) \text{ (By commutative law)} \\
 &\equiv (\neg p \vee q) \vee \neg q \text{ (By associative law)} \\
 &\equiv T \vee \neg q \\
 &\equiv T
 \end{aligned}$$

$$p \rightarrow (q \rightarrow p) \equiv T$$

\therefore It is a tautology.

13. Using the truth table check whether the statements $\neg(p \vee q) \vee (\neg p \wedge q)$ and $\neg p$ are logically equivalent.

Solution:

p	q	$s: p \vee q$	$\neg s$	$\neg p$	$t: \neg p \wedge q$	$\neg s \vee t$
T	T	T	F	F	F	F
T	F	T	F	F	F	F
F	T	T	F	T	T	T
F	F	F	T	T	F	T

Hence both statements are logically equivalent.

Hint: $p \rightarrow q \equiv \neg p \vee q$

14. Prove $p \rightarrow (q \rightarrow r) \equiv (p \wedge q) \rightarrow r$ without using truth table.

Solution:

$$\begin{aligned}
 p \rightarrow (q \rightarrow r) &\equiv p \rightarrow (\neg q \vee r) \\
 &\equiv \neg p \vee (\neg q \vee r) \\
 &\equiv (\neg p \vee \neg q) \vee r \text{ (By associative law)} \\
 &\equiv \neg(p \wedge q) \vee r \text{ (by De Morgan's law)} \\
 p \rightarrow (q \rightarrow r) &\equiv (p \wedge q) \rightarrow r
 \end{aligned}$$

Hence proved.

15. Prove that $p \rightarrow (\neg q \vee r) \equiv \neg p \vee (\neg q \vee r)$ using truth table.

Solution:

p	q	r	$\neg p$	$\neg q$	$s:$ $\neg q \vee r$	$t:$ $p \rightarrow s$	$u:$ $\neg p \vee s$
T	T	T	F	F	T	T	T
T	T	F	F	F	F	F	F
T	F	T	F	T	T	T	T
T	F	F	F	T	T	T	T
F	T	T	T	F	T	T	T
F	T	F	T	F	F	T	T
F	F	T	T	T	T	T	T
F	F	F	T	T	T	T	T

From the table, $p \rightarrow (\neg q \vee r) \equiv \neg p \vee (\neg q \vee r)$